Initial assumption on data: integer or capability in-region (#44)
Squashed commit of the following:

commit dacc631aafa73b29be0af4a9c91e6a6119678dd5
Author: June Rousseau <june.rousseau@cs.au.dk>
Date:   Tue Dec 16 11:29:08 2025 +0100

    Simplify compartment allocation world update: introduce `std_update_compartment`

commit fddb5f16ed58134698acaf2ec7e2e35f912c0ac7
Author: June Rousseau <june.rousseau@cs.au.dk>
Date:   Tue Dec 16 10:13:28 2025 +0100

    Interp of imports as post-condition of `alloc_compartment_interp`

commit 6707cfbd369e4b7efe237b64b0a6556cdab79d27
Author: June Rousseau <june.rousseau@cs.au.dk>
Date:   Tue Dec 16 09:38:42 2025 +0100

    Better formulation of `alloc_compartment_interp`

commit 217c1e872213cb5ef7ff758b66e9ab68b5b2a0f0
Author: June Rousseau <june.rousseau@cs.au.dk>
Date:   Tue Dec 16 00:55:12 2025 +0100

    Simplify even more

commit 63be375c5dc2836104ade3a4f94484981850be6b
Author: June Rousseau <june.rousseau@cs.au.dk>
Date:   Tue Dec 16 00:34:06 2025 +0100

    Weaken data assumption to in_region + nice lemma for initialising the world and showing interp of adversary

theories/case_studies/compartment_layout.v
@@ -598,4 +598,15 @@ Section CmptLayout.
     solve_addr.
   Qed.
 
+  Definition in_region (w : Word) (b e : Addr) :=
+    match w with
+    | WSealable (SCap p Global b' e' a) =>
+        PermFlowsTo p RW (* at most RW capability: excludes WL, excludes XSR *)
+        ∧ (b <= b')%a /\ (e' <= e)%a (* in between the bounds *)
+    | _ => False
+    end.
+
+  Definition is_initial_data_word (B_cmpt : cmpt) :=
+    (fun w => is_z w ∨ in_region w (cmpt_b_cgp B_cmpt) (cmpt_e_cgp B_cmpt)).
+
 End CmptLayout.
