theories/model/region_invariants_allocation.v
@@ -3,6 +3,8 @@ From iris.proofmode Require Import proofmode.
 From stdpp Require Import list_relations.
 From cap_machine Require Export region_invariants multiple_updates.
 From cap_machine Require Import seal_store logrel interp_weakening.
+From cap_machine Require Import switcher.
+From cap_machine Require Import compartment_layout mkregion_helpers stdpp_extra disjoint_regions_tactics.
 Import uPred.
 
 Section region_alloc.
@@ -667,15 +669,19 @@ Section region_alloc.
     sts_full_world W C
     -∗ region W C
     -∗ ([∗ list] k;v ∈ l1;l2, k ↦ₐ v)
-    -∗ ([∗ list] v ∈ l2,
-          (([∗ list] k ∈ l1, rel C k p φ) -∗ φ ((std_update_multiple W l1 Permanent), C, v))
-          ∗ future_priv_mono C φ v)
+    -∗ (
+         ([∗ list] k ∈ l1, rel C k p φ)
+         -∗ ([∗ list] v ∈ l2,
+               (φ ((std_update_multiple W l1 Permanent), C, v)) ∗ future_priv_mono C φ v)
+       )
 
     ={E}=∗
 
     region (std_update_multiple W l1 Permanent) C
+    ∗ sts_full_world (std_update_multiple W l1 Permanent) C
     ∗ ([∗ list] k ∈ l1, rel C k p φ)
-    ∗ sts_full_world (std_update_multiple W l1 Permanent) C.
+    ∗ ([∗ list] v ∈ l2,
+               (φ ((std_update_multiple W l1 Permanent), C, v)) ∗ future_priv_mono C φ v).
   Proof.
     iIntros (HNoDup Hp Hl1) "Hsts Hreg Hl".
     iMod (extend_region_perm_sepL2_open_ind E W C [] l1 l2 p φ with "[Hsts] [Hreg] [Hl]") as
@@ -685,16 +691,583 @@ Section region_alloc.
     { by rewrite -region_open_nil. }
     { cbn; iFrame "Hrel Hsts".
       iIntros "Hφ".
-      iDestruct (big_sepL_sep with "Hφ") as "[Hφ Hmono]".
-      iAssert ([∗ list] y2 ∈ l2, φ (std_update_multiple W l1 Permanent, C, y2))%I as "#Hφ'".
-      { iClear "Hreg Hl Hmono".
-        iInduction (l2) as [|x l2]; first done.
-        iDestruct "Hφ" as "[H1 H2]".
-        iDestruct ("H1" with "Hrel") as "$".
-        iApply ("IHl2" with "H2"); auto.
-      }
+      iDestruct ("Hφ" with "Hrel") as "#Hφ".
+      iFrame "#".
+      iDestruct (big_sepL_sep with "Hφ") as "[Hφ' Hmono]".
       iMod (region_close_many with "Hrel Hreg Hl Hφ' Hmono"); eauto.
     }
   Qed.
 
 End region_alloc.
+
+
+Section region_alloc_cmpt.
+  Context
+    {Σ:gFunctors}
+    {ceriseg:ceriseG Σ} {sealsg: sealStoreG Σ}
+    {Cname : CmptNameG}
+    {stsg : STSG Addr region_type Σ} {heapg : heapGS Σ}
+    {nainv: logrel_na_invs Σ}
+    {cstackg : CSTACKG Σ}
+    `{MP: MachineParameters}
+  .
+
+  Definition std_update_compartment (W : WORLD) (C_cmpt : cmpt) :=
+    let imports_addrs := finz.seq_between (cmpt_b_pcc C_cmpt) (cmpt_a_code C_cmpt) in
+    let code_addrs := finz.seq_between (cmpt_a_code C_cmpt) (cmpt_e_pcc C_cmpt) in
+    let data_addrs := finz.seq_between (cmpt_b_cgp C_cmpt) (cmpt_e_cgp C_cmpt) in
+    let Wcode := std_update_multiple W code_addrs Permanent in
+    let Wdata := std_update_multiple Wcode data_addrs Permanent in
+    std_update_multiple Wdata imports_addrs Permanent.
+
+  Lemma std_update_compartment_pub (W : WORLD) (C_cmpt : cmpt) :
+    let imports_addrs := finz.seq_between (cmpt_b_pcc C_cmpt) (cmpt_a_code C_cmpt) in
+    let code_addrs := finz.seq_between (cmpt_a_code C_cmpt) (cmpt_e_pcc C_cmpt) in
+    let data_addrs := finz.seq_between (cmpt_b_cgp C_cmpt) (cmpt_e_cgp C_cmpt) in
+    Forall (λ k, std W !! k = None) imports_addrs →
+    Forall (λ k, std W !! k = None) code_addrs →
+    Forall (λ k, std W !! k = None) data_addrs →
+    related_sts_pub_world W (std_update_compartment W C_cmpt).
+  Proof.
+    intros * Himports Hcode Hdata.
+    rewrite !Forall_forall in Himports, Hcode, Hdata.
+    set (W2 := std_update_multiple W (finz.seq_between (cmpt_a_code C_cmpt) (cmpt_e_pcc C_cmpt)) Permanent).
+    assert (related_sts_pub_world W W2) as Hrelated_pub_W_W2.
+    { apply related_sts_pub_update_multiple.
+      apply Forall_forall.
+      intros a Ha.
+      by apply Hcode in Ha; rewrite -not_elem_of_dom in Ha.
+    }
+    set (W3 := std_update_multiple W2 (finz.seq_between (cmpt_b_cgp C_cmpt) (cmpt_e_cgp C_cmpt)) Permanent).
+    assert (related_sts_pub_world W2 W3) as Hrelated_pub_W2_W3.
+    { apply related_sts_pub_update_multiple.
+      apply Forall_forall.
+      intros a Ha.
+      assert (a ∉ dom W.1)
+        as Hadom by (by apply Hdata in Ha; rewrite -not_elem_of_dom in Ha).
+      subst W2.
+      intro Ha'.
+      apply elem_of_dom_std_multiple_update in Ha' as [Ha' | Ha']; last done.
+      pose proof (cmpt_cgp_disjoint C_cmpt) as Hdisjoint.
+      apply map_disjoint_dom_1 in Hdisjoint.
+      rewrite /cmpt_pcc_mregion dom_union_L in Hdisjoint.
+      rewrite disjoint_union_l in Hdisjoint.
+      destruct Hdisjoint as [_ Hdisjoint].
+      pose proof (cmpt_data_size C_cmpt) as Hsize_data.
+      pose proof (cmpt_code_size C_cmpt) as Hsize_code.
+      rewrite !dom_mkregion_eq in Hdisjoint; auto.
+      apply list_to_set_disj_2 in Hdisjoint.
+      rewrite /disjoint /set_disjoint_instance in Hdisjoint.
+      apply (Hdisjoint a); auto.
+    }
+    set (W4 := std_update_multiple W3 (finz.seq_between (cmpt_b_pcc C_cmpt) (cmpt_a_code C_cmpt))
+                 Permanent).
+    assert (Forall (fun a => a ∉ dom (std W3))
+              (finz.seq_between (cmpt_b_pcc C_cmpt) (cmpt_a_code C_cmpt))) as Himports_W3.
+    { apply Forall_forall; intros a Ha; cbn.
+      assert (a ∉ dom W.1)
+        as Hadom by (by apply Himports in Ha; rewrite -not_elem_of_dom in Ha).
+      rewrite not_elem_of_dom.
+      pose proof (cmpt_import_size C_cmpt) as H.
+      rewrite std_sta_update_multiple_lookup_same_i; auto.
+      2: {
+        pose proof (cmpt_cgp_disjoint C_cmpt) as Hdisjoint.
+        apply map_disjoint_dom_1 in Hdisjoint.
+        rewrite /cmpt_pcc_mregion dom_union_L in Hdisjoint.
+        rewrite disjoint_union_l in Hdisjoint.
+        destruct Hdisjoint as [H1 _].
+        pose proof (cmpt_data_size C_cmpt) as Hsize_data.
+        pose proof (cmpt_import_size C_cmpt) as Hsize_imports.
+        pose proof (cmpt_code_size C_cmpt) as Hsize_code.
+        rewrite !dom_mkregion_eq in H1; auto.
+        apply list_to_set_disj_2 in H1.
+        apply H1 in Ha; eauto.
+      }
+      rewrite std_sta_update_multiple_lookup_same_i; auto.
+      {  pose proof (cmpt_code_disjoint C_cmpt) as Hdis.
+         apply map_disjoint_dom_1 in Hdis.
+        pose proof (cmpt_import_size C_cmpt) as Hsize_imports.
+        pose proof (cmpt_code_size C_cmpt) as Hsize_code.
+        rewrite !dom_mkregion_eq in Hdis; auto.
+        apply list_to_set_disj_2 in Hdis.
+        apply Hdis in Ha; eauto.
+      }
+    }
+    assert (related_sts_pub_world W3 W4) as Hrelated_pub_W3_W4.
+    { apply related_sts_pub_update_multiple; auto. }
+    eapply related_sts_pub_trans_world; eauto.
+    eapply related_sts_pub_trans_world; eauto.
+  Qed.
+
+  Lemma switcher_cmpt_disjoint_std_update_compartment
+    `{switcher_layout : (@switcherLayout MP)}
+    (W : WORLD) (C_cmpt : cmpt) (switcher_cmpt : cmptSwitcher) (a : Addr) :
+    a ∈ finz.seq_between (b_stack switcher_cmpt) (e_stack switcher_cmpt) ->
+    switcher_cmpt_disjoint C_cmpt switcher_cmpt ->
+    std W !! a = None ->
+    std (std_update_compartment W C_cmpt) !! a = None.
+  Proof.
+    intros Ha Hc Ha_W.
+    pose proof (cmpt_import_size C_cmpt) as H.
+    pose proof (cmpt_code_size C_cmpt) as H'.
+    rewrite std_sta_update_multiple_lookup_same_i.
+    2: {
+      intro Hcontra.
+      assert (a ∈ finz.seq_between (cmpt_b_pcc C_cmpt) (cmpt_e_pcc C_cmpt)).
+      {
+        apply elem_of_finz_seq_between.
+        apply elem_of_finz_seq_between in Hcontra.
+        solve_addr+H H' Hcontra.
+      }
+      apply (Hc a).
+      + rewrite /cmpt_switcher_region.
+        eapply elem_of_union;eauto.
+      + eapply elem_of_union;eauto.
+        left; eapply elem_of_union;eauto.
+    }
+    rewrite std_sta_update_multiple_lookup_same_i.
+    2: { intro Hcontra.
+         apply (Hc a); eauto.
+         + eapply elem_of_union;eauto.
+         + eapply elem_of_union;eauto.
+           left;eapply elem_of_union;eauto.
+    }
+    rewrite std_sta_update_multiple_lookup_same_i; first done.
+    intro Hcontra.
+    apply (Hc a); eauto.
+    + eapply elem_of_union;eauto.
+    + eapply elem_of_union;eauto.
+      left;eapply elem_of_union;eauto.
+      left.
+      rewrite !elem_of_finz_seq_between in Hcontra |- *.
+      solve_addr+H H' Hcontra.
+  Qed.
+
+  Lemma alloc_compartment_interp_rel (E : coPset) (W : WORLD) ( C_cmpt : cmpt ) (C : CmptName)  :
+    let imports_addrs := finz.seq_between (cmpt_b_pcc C_cmpt) (cmpt_a_code C_cmpt) in
+    let code_addrs := finz.seq_between (cmpt_a_code C_cmpt) (cmpt_e_pcc C_cmpt) in
+    let data_addrs := finz.seq_between (cmpt_b_cgp C_cmpt) (cmpt_e_cgp C_cmpt) in
+    let pcc_cap := (WCap RX Global (cmpt_b_pcc C_cmpt) (cmpt_e_pcc C_cmpt) (cmpt_b_pcc C_cmpt)%a) in
+    let cgp_cap := (WCap RW Global (cmpt_b_cgp C_cmpt) (cmpt_e_cgp C_cmpt) (cmpt_b_cgp C_cmpt)%a) in
+    let Wfinal := std_update_compartment W C_cmpt in
+
+    Forall (λ k, std W !! k = None) imports_addrs →
+    Forall (λ k, std W !! k = None) code_addrs →
+    Forall (λ k, std W !! k = None) data_addrs →
+
+    Forall (λ w : Word, is_z w) (cmpt_code C_cmpt) ->
+    Forall (is_initial_data_word C_cmpt) (cmpt_data C_cmpt) ->
+
+    ([∗ list] k;v ∈ imports_addrs ; cmpt_imports C_cmpt, k ↦ₐ v) -∗
+    ([∗ list] k;v ∈ code_addrs ; cmpt_code C_cmpt, k ↦ₐ v) -∗
+    ([∗ list] k;v ∈ data_addrs ; cmpt_data C_cmpt, k ↦ₐ v) -∗
+
+    (
+      (
+        ([∗ list] k ∈ (imports_addrs++code_addrs), rel C k RX interpC)
+        ∗ ([∗ list] k ∈ (data_addrs), rel C k RW interpC)
+      )
+      -∗
+      ([∗ list] v ∈ cmpt_imports C_cmpt, interpC (Wfinal, C, v) ∗ future_priv_mono C interpC v)
+    ) -∗
+
+    sts_full_world W C -∗
+    region W C
+
+    ={E}=∗
+
+    sts_full_world Wfinal C
+    ∗ region Wfinal C
+    ∗ interp Wfinal C pcc_cap
+    ∗ interp Wfinal C cgp_cap
+    ∗ ([∗ list] v ∈ cmpt_imports C_cmpt, interp Wfinal C v)
+  .
+  Proof.
+    intros * Himports Hcode Hdata C_code C_data.
+    iIntros "HC_imports HC_code HC_data Himport_interp Hsts_C Hr_C".
+
+    iMod (extend_region_perm_sepL2 _ W C
+            code_addrs (cmpt_code C_cmpt)
+            RX interpC
+           with "Hsts_C Hr_C [HC_code]") as "(Hr_C & #HC_code & Hsts_C)".
+    { done. }
+    { auto. }
+    {
+      iApply (big_sepL2_mono ((fun (_ : nat) (k : finz.finz MemNum) (v : Word) =>
+                                 pointsto k (DfracOwn (pos_to_Qp 1)) v)) with "[HC_code]").
+      - intros k v1 v2 Hv1 Hv2. cbn. iIntros; iFrame.
+        pose proof (Forall_lookup_1 _ _ _ _ C_code Hv2) as Hncap.
+        destruct v2; [| by inversion Hncap..].
+        rewrite /interpC /safeC fixpoint_interp1_eq /=.
+        iSplit; eauto.
+        iApply future_priv_mono_interp_z.
+      - iFrame.
+    }
+
+    iMod (extend_region_perm_sepL2_open _ _ C
+            data_addrs
+            (cmpt_data C_cmpt)
+            RW interpC
+           with "Hsts_C Hr_C [HC_data] []") as "(Hr_C & Hsts_C & #HC_data & _)".
+    { apply finz_seq_between_NoDup. }
+    { done. }
+    { apply Forall_forall. intros a Ha.
+      rewrite std_sta_update_multiple_lookup_same_i; auto.
+      { by rewrite Forall_forall in Hdata; apply Hdata in Ha. }
+      pose proof (cmpt_cgp_disjoint C_cmpt) as Hdisjoint.
+      apply map_disjoint_dom_1 in Hdisjoint.
+      rewrite /cmpt_pcc_mregion dom_union_L in Hdisjoint.
+      rewrite disjoint_union_l in Hdisjoint.
+      destruct Hdisjoint as [_ Hdisjoint].
+      pose proof (cmpt_data_size C_cmpt) as Hsize_data.
+      pose proof (cmpt_code_size C_cmpt) as Hsize_code.
+      rewrite !dom_mkregion_eq in Hdisjoint; auto.
+      apply list_to_set_disj_2 in Hdisjoint.
+      rewrite /disjoint /set_disjoint_instance in Hdisjoint.
+      intro Ha'.
+      apply (Hdisjoint a); auto.
+    }
+    {
+      iApply (big_sepL2_mono ((fun (_ : nat) (k : finz.finz MemNum) (v : Word) =>
+                                 pointsto k (DfracOwn (pos_to_Qp 1)) v)) with "HC_data").
+      intros k v1 v2 Hv1 Hv2. iIntros; iFrame.
+    }
+    {
+      iClear "#".
+      clear -C_data.
+      generalize dependent (cmpt_data C_cmpt); iIntros (l Hl).
+      iIntros "#Hrels".
+      iInduction (l) as [| w l] "IH"; first done.
+      cbn.
+      apply Forall_cons in Hl; destruct Hl as [Hw Hl].
+      iSplitL; last (iApply "IH"; eauto).
+      destruct w as [| [|] | |] ; cbn in Hw; destruct Hw as [Hw|Hw]; cbn in Hw; try done
+      ; [|destruct g ; last done].
+      - iSplit; last iApply future_priv_mono_interp_z.
+        by rewrite /interpC /safeC fixpoint_interp1_eq /=.
+      - iSplit; last iApply future_priv_mono_interp_global.
+        rewrite /interpC /safeC fixpoint_interp1_eq interp1_eq.
+        destruct Hw as (Hp & Hb & He).
+        destruct (isO p) eqn:HpO; first done.
+        destruct (has_sreg_access p) eqn:HpXSR.
+        { destruct p as [ [] w dl dro ]; cbn in *; done. }
+        replace (isWL p) with false; cycle 1.
+        { destruct p as [ rx [] dl dro ]; cbn in *; auto.
+          rewrite !andb_True in Hp.
+          destruct Hp as [ [ [] ] ]; done.
+        }
+        iSplit; last done.
+        iApply big_sepL_forall; cbn.
+        iIntros (k a' Ha').
+        apply elem_of_list_lookup_2, elem_of_finz_seq_between in Ha'.
+        assert ((cmpt_b_cgp C_cmpt) <= a' < (cmpt_e_cgp C_cmpt))%a as Ha'' by solve_addr.
+        apply elem_of_finz_seq_between in Ha''.
+        iDestruct (big_sepL_elem_of with "Hrels") as "Hrel_a'"; eauto.
+        assert (
+            (std_update_multiple (std_update_multiple W code_addrs Permanent) data_addrs Permanent).1
+              !! a' = Some Permanent
+          ) as Ha'_W.
+        { by apply std_sta_update_multiple_lookup_in_i. }
+        iExists RW, interp; cbn.
+        iSplit; first done.
+        iSplit; first (iPureIntro; apply persistent_cond_interp).
+        iSplit; first iFrame "#".
+        iSplit; first iApply zcond_interp.
+        iSplit; first iApply rcond_interp.
+        iSplit; first iApply wcond_interp.
+        iSplit; first iApply monoReq_interp; eauto.
+    }
+
+    iMod (extend_region_perm_sepL2_open _ _ C
+            imports_addrs
+            (cmpt_imports C_cmpt)
+            RX interpC
+           with "Hsts_C Hr_C HC_imports [Himport_interp]") as "(Hr_C & Hsts_C & #HC_imports & Hinterp_imports)".
+    { apply finz_seq_between_NoDup. }
+    { done. }
+    { apply Forall_forall.
+      intros a Ha.
+      rewrite std_sta_update_multiple_lookup_same_i; auto.
+      + rewrite std_sta_update_multiple_lookup_same_i; auto.
+        { by rewrite Forall_forall in Himports; apply Himports in Ha. }
+        pose proof (cmpt_import_size C_cmpt) as HC.
+        apply not_elem_of_finz_seq_between.
+        subst imports_addrs.
+        rewrite elem_of_finz_seq_between in Ha.
+        solve_addr+HC Ha.
+      + pose proof (cmpt_disjointness C_cmpt) as HC.
+        apply disjoint_regions_tactics.disjoint_list_cons in HC
+        ; destruct HC as [HC _].
+        rewrite union_list_cons in HC.
+        cbn in HC.
+        assert (
+            finz.seq_between (cmpt_b_pcc C_cmpt) (cmpt_e_pcc C_cmpt)
+              ## finz.seq_between (cmpt_b_cgp C_cmpt) (cmpt_e_cgp C_cmpt)
+          ) as HC' by set_solver+HC
+        ; clear HC.
+        intro Hcontra ; eapply HC'; eauto.
+        pose proof (cmpt_import_size C_cmpt) as H.
+        pose proof (cmpt_code_size C_cmpt) as H'.
+        rewrite elem_of_finz_seq_between in Ha.
+        apply elem_of_finz_seq_between; solve_addr+H H' Ha.
+    }
+    { iIntros "#HC_imports".
+      iApply "Himport_interp"; iFrame "#".
+    }
+    iDestruct (big_sepL_sep with "Hinterp_imports") as "[$ _]".
+    iFrame.
+    iModIntro.
+    iDestruct (big_sepL_app _ imports_addrs code_addrs with "[$HC_imports $HC_code]") as "HC_PCC".
+    rewrite -finz_seq_between_split.
+    2: {
+      pose proof (cmpt_import_size C_cmpt) as HC.
+      pose proof (cmpt_code_size C_cmpt) as HC'.
+      solve_addr.
+    }
+
+    iSplit.
+    - iEval (rewrite fixpoint_interp1_eq /=).
+      iApply big_sepL_intro; iModIntro.
+      iIntros (k a Ha).
+      iExists RX, interp.
+      iEval (cbn).
+      iSplit; first done.
+      iSplit; first (iPureIntro ; by apply persistent_cond_interp).
+      iSplit.
+      { apply elem_of_list_lookup_2 in Ha.
+        iApply (big_sepL_elem_of with "HC_PCC"); eauto.
+      }
+      iSplit; first (iNext ; by iApply zcond_interp).
+      iSplit; first (iNext ; by iApply rcond_interp).
+      iSplit; first done.
+      assert ((std Wfinal) !! a = Some Permanent).
+      {
+        subst Wfinal.
+        apply elem_of_list_lookup_2 in Ha.
+        rewrite (finz_seq_between_split _ (cmpt_a_code C_cmpt)) in Ha.
+        2: {
+          pose proof (cmpt_import_size C_cmpt) as HC.
+          pose proof (cmpt_code_size C_cmpt) as HC'.
+          solve_addr.
+        }
+        rewrite elem_of_app in Ha.
+        destruct Ha as [ Ha | Ha ]; simplify_eq.
+        + rewrite std_sta_update_multiple_lookup_in_i; auto; set_solver+.
+        + rewrite std_sta_update_multiple_lookup_same_i; cycle 1.
+          { pose proof (cmpt_import_size C_cmpt) as HC.
+            pose proof (cmpt_code_size C_cmpt) as HC'.
+            apply elem_of_finz_seq_between in Ha.
+            apply not_elem_of_finz_seq_between.
+            solve_addr.
+          }
+          rewrite std_sta_update_multiple_lookup_same_i; cycle 1.
+          { intro Hcontra.
+            assert (
+                (finz.seq_between (cmpt_a_code C_cmpt) (cmpt_e_pcc C_cmpt))
+                  ##
+                  (finz.seq_between (cmpt_b_cgp C_cmpt) (cmpt_e_cgp C_cmpt))
+              ) as Hdis; last set_solver+Ha Hcontra Hdis.
+            clear.
+            pose proof (cmpt_cgp_disjoint C_cmpt) as Hdis.
+            rewrite /cmpt_pcc_mregion /cmpt_cgp_mregion in Hdis.
+            rewrite -/(cmpt_pcc_mregion C_cmpt) -/(cmpt_cgp_mregion C_cmpt) in Hdis.
+            rewrite map_disjoint_dom in Hdis.
+            rewrite dom_cmpt_pcc_mregion dom_cmpt_cgp_mregion /cmpt_pcc_region /cmpt_cgp_region in Hdis.
+            rewrite -list_to_set_disj in Hdis.
+            assert (
+                finz.seq_between (cmpt_a_code C_cmpt) (cmpt_e_pcc C_cmpt) ⊆ finz.seq_between (cmpt_b_pcc C_cmpt) (cmpt_e_pcc C_cmpt)
+              ); last set_solver.
+            intros a Ha.
+            rewrite !elem_of_finz_seq_between in Ha |- *.
+            pose proof (cmpt_import_size C_cmpt).
+            solve_addr.
+          }
+          rewrite std_sta_update_multiple_lookup_in_i; auto; set_solver+.
+      }
+      iSplit; last done.
+      iApply (monoReq_interp _ _ _ _ Permanent); done.
+    - iEval (rewrite fixpoint_interp1_eq /=).
+      iApply big_sepL_intro; iModIntro.
+      iIntros (k a Ha).
+      iExists RW, interp.
+      iEval (cbn).
+      iSplit; first done.
+      iSplit; first (iPureIntro ; by apply persistent_cond_interp).
+      rewrite (big_sepL_lookup _ (finz.seq_between (cmpt_b_cgp C_cmpt) (cmpt_e_cgp C_cmpt))
+                 k a); eauto.
+      iFrame "HC_data".
+      iSplit; first (iNext ; by iApply zcond_interp).
+      iSplit; first (iNext ; by iApply rcond_interp).
+      iSplit; first (iNext ; by iApply wcond_interp).
+      assert ((std Wfinal) !! a = Some Permanent).
+      { subst Wfinal.
+        apply elem_of_list_lookup_2 in Ha.
+        assert (a ∉ imports_addrs).
+        { clear -Ha.
+          pose proof (cmpt_disjointness C_cmpt) as Hdis.
+          apply disjoint_list_cons in Hdis as [Hdis _].
+          rewrite union_list_cons disjoint_union_r in Hdis.
+          destruct Hdis as [Hdis _].
+          intro Hcontra.
+          assert ( a ∈ finz.seq_between (cmpt_b_pcc C_cmpt) (cmpt_e_pcc C_cmpt))
+          ; last set_solver.
+          pose proof (cmpt_import_size C_cmpt) as Hsize.
+          pose proof (cmpt_code_size C_cmpt).
+          apply elem_of_finz_seq_between in Hcontra.
+          apply elem_of_finz_seq_between.
+          solve_addr.
+        }
+        repeat (rewrite std_sta_update_multiple_lookup_same_i; last done).
+        rewrite std_sta_update_multiple_lookup_in_i; auto.
+      }
+      iSplit; last done.
+      iApply (monoReq_interp _ _ _ _ Permanent); done.
+  Qed.
+
+  Lemma alloc_compartment_interp (E : coPset) (W : WORLD) ( C_cmpt : cmpt ) (C : CmptName)  :
+    let imports_addrs := finz.seq_between (cmpt_b_pcc C_cmpt) (cmpt_a_code C_cmpt) in
+    let code_addrs := finz.seq_between (cmpt_a_code C_cmpt) (cmpt_e_pcc C_cmpt) in
+    let data_addrs := finz.seq_between (cmpt_b_cgp C_cmpt) (cmpt_e_cgp C_cmpt) in
+    let pcc_cap := (WCap RX Global (cmpt_b_pcc C_cmpt) (cmpt_e_pcc C_cmpt) (cmpt_b_pcc C_cmpt)%a) in
+    let cgp_cap := (WCap RW Global (cmpt_b_cgp C_cmpt) (cmpt_e_cgp C_cmpt) (cmpt_b_cgp C_cmpt)%a) in
+    let Wfinal := std_update_compartment W C_cmpt in
+
+    Forall (λ k, std W !! k = None) imports_addrs →
+    Forall (λ k, std W !! k = None) code_addrs →
+    Forall (λ k, std W !! k = None) data_addrs →
+
+    Forall (λ w : Word, is_z w) (cmpt_code C_cmpt) ->
+    Forall (is_initial_data_word C_cmpt) (cmpt_data C_cmpt) ->
+
+    ([∗ list] k;v ∈ imports_addrs ; cmpt_imports C_cmpt, k ↦ₐ v) -∗
+    ([∗ list] k;v ∈ code_addrs ; cmpt_code C_cmpt, k ↦ₐ v) -∗
+    ([∗ list] k;v ∈ data_addrs ; cmpt_data C_cmpt, k ↦ₐ v) -∗
+    (
+      (interp Wfinal C pcc_cap ∗ interp Wfinal C cgp_cap)
+      -∗
+      ([∗ list] v ∈ cmpt_imports C_cmpt, interpC (Wfinal, C, v) ∗ future_priv_mono C interpC v)
+    )
+    -∗
+
+    sts_full_world W C -∗
+    region W C
+
+    ={E}=∗
+
+    sts_full_world Wfinal C
+    ∗ region Wfinal C
+    ∗ interp Wfinal C pcc_cap
+    ∗ interp Wfinal C cgp_cap
+    ∗ ([∗ list] v ∈ cmpt_imports C_cmpt, interp Wfinal C v)
+  .
+  Proof.
+    intros * Himports Hcode Hdata C_code C_data.
+    iIntros "HC_imports HC_code HC_data Himport_interp Hsts_C Hr_C".
+    iApply (alloc_compartment_interp_rel with "[$] [$] [$] [Himport_interp] [$] [$]"); eauto.
+    iIntros "[#Hrel_pcc #Hrel_data]".
+    iApply "Himport_interp".
+    iSplit.
+    - iEval (rewrite fixpoint_interp1_eq /=).
+      iApply big_sepL_intro; iModIntro.
+      iIntros (ka a Ha).
+      iExists RX, interp.
+      iEval (cbn).
+      iSplit; first done.
+      iSplit; first (iPureIntro ; by apply persistent_cond_interp).
+      iSplit.
+      { apply elem_of_list_lookup_2 in Ha.
+        iApply (big_sepL_elem_of with "Hrel_pcc"); eauto.
+        rewrite -finz_seq_between_split;auto.
+        pose proof (cmpt_import_size C_cmpt) as HC.
+        pose proof (cmpt_code_size C_cmpt) as HC'.
+        solve_addr.
+      }
+      iSplit; first (iNext ; by iApply zcond_interp).
+      iSplit; first (iNext ; by iApply rcond_interp).
+      iSplit; first done.
+      assert ((std Wfinal) !! a = Some Permanent).
+      {
+        subst Wfinal.
+        apply elem_of_list_lookup_2 in Ha.
+        rewrite (finz_seq_between_split _ (cmpt_a_code C_cmpt)) in Ha.
+        2: {
+          pose proof (cmpt_import_size C_cmpt) as HC.
+          pose proof (cmpt_code_size C_cmpt) as HC'.
+          solve_addr.
+        }
+        rewrite elem_of_app in Ha.
+        destruct Ha as [ Ha | Ha ]; simplify_eq.
+        + rewrite std_sta_update_multiple_lookup_in_i; auto; set_solver+.
+        + rewrite std_sta_update_multiple_lookup_same_i; cycle 1.
+          { pose proof (cmpt_import_size C_cmpt) as HC.
+            pose proof (cmpt_code_size C_cmpt) as HC'.
+            apply elem_of_finz_seq_between in Ha.
+            apply not_elem_of_finz_seq_between.
+            solve_addr.
+          }
+          rewrite std_sta_update_multiple_lookup_same_i; cycle 1.
+          { intro Hcontra.
+            assert (
+                (finz.seq_between (cmpt_a_code C_cmpt) (cmpt_e_pcc C_cmpt))
+                  ##
+                  (finz.seq_between (cmpt_b_cgp C_cmpt) (cmpt_e_cgp C_cmpt))
+              ) as Hdis; last set_solver+Ha Hcontra Hdis.
+            clear.
+            pose proof (cmpt_cgp_disjoint C_cmpt) as Hdis.
+            rewrite /cmpt_pcc_mregion /cmpt_cgp_mregion in Hdis.
+            rewrite -/(cmpt_pcc_mregion C_cmpt) -/(cmpt_cgp_mregion C_cmpt) in Hdis.
+            rewrite map_disjoint_dom in Hdis.
+            rewrite dom_cmpt_pcc_mregion dom_cmpt_cgp_mregion /cmpt_pcc_region /cmpt_cgp_region in Hdis.
+            rewrite -list_to_set_disj in Hdis.
+            assert (
+                finz.seq_between (cmpt_a_code C_cmpt) (cmpt_e_pcc C_cmpt) ⊆ finz.seq_between (cmpt_b_pcc C_cmpt) (cmpt_e_pcc C_cmpt)
+              ); last set_solver.
+            intros a Ha.
+            rewrite !elem_of_finz_seq_between in Ha |- *.
+            pose proof (cmpt_import_size C_cmpt).
+            solve_addr.
+          }
+          rewrite std_sta_update_multiple_lookup_in_i; auto; set_solver+.
+      }
+      iSplit; last done.
+      iApply (monoReq_interp _ _ _ _ Permanent); done.
+    - iEval (rewrite fixpoint_interp1_eq /=).
+      iApply big_sepL_intro; iModIntro.
+      iIntros (ka a Ha).
+      iExists RW, interp.
+      iEval (cbn).
+      iSplit; first done.
+      iSplit; first (iPureIntro ; by apply persistent_cond_interp).
+      rewrite (big_sepL_lookup _ (finz.seq_between (cmpt_b_cgp C_cmpt) (cmpt_e_cgp C_cmpt))
+                 ka a); eauto.
+      iFrame "Hrel_data".
+      iSplit; first (iNext ; by iApply zcond_interp).
+      iSplit; first (iNext ; by iApply rcond_interp).
+      iSplit; first (iNext ; by iApply wcond_interp).
+      assert ((std Wfinal) !! a = Some Permanent).
+      { subst Wfinal.
+        apply elem_of_list_lookup_2 in Ha.
+        assert (a ∉ imports_addrs).
+        { clear -Ha.
+          pose proof (cmpt_disjointness C_cmpt) as Hdis.
+          apply disjoint_list_cons in Hdis as [Hdis _].
+          rewrite union_list_cons disjoint_union_r in Hdis.
+          destruct Hdis as [Hdis _].
+          intro Hcontra.
+          assert ( a ∈ finz.seq_between (cmpt_b_pcc C_cmpt) (cmpt_e_pcc C_cmpt))
+          ; last set_solver.
+          pose proof (cmpt_import_size C_cmpt) as Hsize.
+          pose proof (cmpt_code_size C_cmpt).
+          apply elem_of_finz_seq_between in Hcontra.
+          apply elem_of_finz_seq_between.
+          solve_addr.
+        }
+        repeat (rewrite std_sta_update_multiple_lookup_same_i; last done).
+        rewrite std_sta_update_multiple_lookup_in_i; auto.
+      }
+      iSplit; last done.
+      iApply (monoReq_interp _ _ _ _ Permanent); done.
+  Qed.
+
+
+End region_alloc_cmpt.
